\section*{Problem 1}
\addcontentsline{toc}{section}{Problem 1}

\textbf{Statement:}

$\quad P(\overline{A}) = \frac{3}{4}, \quad P(B|A) = \frac{1}{3}; \text{ find } P(A\cap\overline{B})$

\noindent\textbf{Solution:}

By complement rule we have $P(\overline{A}) = 1 - P(A)$:

\begin{equation*}
    P(A) = 1 - P(\overline{A}) = 1 - \frac{3}{4} = \frac{1}{4}
\end{equation*}

By conditional probability definition we have $P(B|A) = \frac{P(A\cap B)}{P(A)}$:

\begin{equation*}
    P(A\cap B) = P(B|A)P(A) = \frac{1}{3} \cdot \frac{1}{4} = \frac{1}{12}
\end{equation*}

By law of total probability we have $P(A) = \sum_{i=1}^n P(A|B_i)P(B_i)$, where
$\bigcup_{i=1}^n B_i = \Omega$ and $B_i \cap B_j = \emptyset$ for $i \neq j$.

So because $B \cup \overline{B} = \Omega$ and $B \cap \overline{B} = \emptyset$ we have:

\begin{equation*}
    \begin{split}
        P(A)                 & = P(A|B)P(B) + P(A|\overline{B})P(\overline{B}) \\
        P(A)                 & = P(A\cap B) + P(A\cap\overline{B})             \\
        P(A\cap\overline{B}) & = P(A) - P(A\cap B)                             \\
        P(A\cap\overline{B}) & = \frac{1}{4} - \frac{1}{12}                    \\
        P(A\cap\overline{B}) & = \frac{1}{6}
    \end{split}
\end{equation*}