\section*{Problem 1}
\addcontentsline{toc}{section}{Problem 1}

Derive formulas how to compute Expectation of second moment, third moment and Dispersion using Generating functions

\textbf{Second Moment}:

We need to calculate the second moment of a random variable \( \xi \), which is defined as:

\[ E(\xi^2) = \sum_{i=0}^{\infty} i^2 \cdot P(\xi = i) \]

Now we have the formula for the generating function of \( \xi \):

\[ G_{\xi}(x) = \sum_{i=0}^{\infty} P(\xi = i) \cdot x^i \]

Let's find the first and second derivatives of \( G_{\xi}(x) \):


\[ G'_{\xi}(x) = \sum_{i=0}^{\infty} i \cdot P(\xi = i) \cdot x^{i-1} \]

\[ G''_{\xi}(x) = \sum_{i=0}^{\infty} i \cdot (i-1) \cdot P(\xi = i) \cdot x^{i-2} \]

Then if we multiply \( G'_\xi(x) \) by \( x \) and \( G''_\xi(x) \) by \( x^2 \), we get:

\[ x \cdot G'_{\xi}(x) = \sum_{i=0}^{\infty} i \cdot P(\xi = i) \cdot x^{i} \]

\[ x^2 \cdot G''_{\xi}(x) = \sum_{i=0}^{\infty} i \cdot (i-1) \cdot P(\xi = i) \cdot x^{i} \]

Now if we add these two equations, we get:

\[ x \cdot G'_{\xi}(x) + x^2 \cdot G''_{\xi}(x) = \sum_{i=0}^{\infty} i \cdot P(\xi = i) \cdot x^{i} + \sum_{i=0}^{\infty} i \cdot (i-1) \cdot P(\xi = i) \cdot x^{i} = \sum_{i=0}^{\infty} i^2 \cdot P(\xi = i) \cdot x^{i} \]

Then replacing $x$ with $1$ we get:

\[ 1 \cdot G'_{\xi}(1) + 1^2 \cdot G''_{\xi}(1) = \sum_{i=0}^{\infty} i^2 \cdot P(\xi = i) \cdot 1^{i} = \sum_{i=0}^{\infty} i^2 \cdot P(\xi = i) \]

So we get:

\[ E(\xi^2) = G'_{\xi}(1) + G''_{\xi}(1) \]

\newpage

\textbf{Third Moment}:

We need to calculate the third moment of a random variable \( \xi \), which is defined as:

\[ E(\xi^3) = \sum_{i=0}^{\infty} i^3 \cdot P(\xi = i) \]

Now we have the formula for the generating function of \( \xi \):

\[ G_{\xi}(x) = \sum_{i=0}^{\infty} P(\xi = i) \cdot x^i \]

Let's find the first, second and third derivatives of \( G_{\xi}(x) \):

\[ G'_{\xi}(x) = \sum_{i=0}^{\infty} i \cdot P(\xi = i) \cdot x^{i-1} \]

\[ G''_{\xi}(x) = \sum_{i=0}^{\infty} i \cdot (i-1) \cdot P(\xi = i) \cdot x^{i-2} \]

\[ G'''_{\xi}(x) = \sum_{i=0}^{\infty} i \cdot (i-1) \cdot (i-2) \cdot P(\xi = i) \cdot x^{i-3} \]

Then if we multiply \( G'_\xi(x) \) by \( x \), \( G''_\xi(x) \) by \( x^2 \) and \( G'''_\xi(x) \) by \( x^3 \), we get:

\[ x \cdot G'_{\xi}(x) = \sum_{i=0}^{\infty} i \cdot P(\xi = i) \cdot x^{i} \]

\[ x^2 \cdot G''_{\xi}(x) = \sum_{i=0}^{\infty} i \cdot (i-1) \cdot P(\xi = i) \cdot x^{i} \]

\[ x^3 \cdot G'''_{\xi}(x) = \sum_{i=0}^{\infty} i \cdot (i-1) \cdot (i-2) \cdot P(\xi = i) \cdot x^{i} \]

Note that if we add the first equation plus three times the second equation plus the third equation, we get:

\[ x \cdot G'_{\xi}(x) + 3 \cdot x^2 \cdot G''_{\xi}(x) + x^3 \cdot G'''_{\xi}(x) = \sum_{i=0}^{\infty} i \cdot P(\xi = i) \cdot x^{i} + \sum_{i=0}^{\infty} 3 \cdot i \cdot (i-1) \cdot P(\xi = i) \cdot x^{i} + \sum_{i=0}^{\infty} i \cdot (i-1) \cdot (i-2) \cdot P(\xi = i) \cdot x^{i} \]

\[ = \sum_{i=0}^{\infty} i^3 \cdot P(\xi = i) \cdot x^{i} \]

Then replacing $x$ with $1$ we get:

\[ 1 \cdot G'_{\xi}(1) + 3 \cdot 1^2 \cdot G''_{\xi}(1) + 1^3 \cdot G'''_{\xi}(1) = \sum_{i=0}^{\infty} i^3 \cdot P(\xi = i) \cdot 1^{i} = \sum_{i=0}^{\infty} i^3 \cdot P(\xi = i) \]

So we get:

\[ E(\xi^3) = G'_{\xi}(1) + 3 \cdot G''_{\xi}(1) + G'''_{\xi}(1) \]

\newpage

\textbf{Dispersion}:

We need to calculate the dispersion of a random variable \( \xi \), which is defined as:

\[ D(\xi) = E(( \xi - E(\xi) )^2) = E(\xi^2 - 2 \cdot \xi \cdot E(\xi) + E(\xi)^2) = E(\xi^2) - 2 \cdot E(\xi) \cdot E(\xi) + E(\xi)^2 = E(\xi^2) - E(\xi)^2 \]

We already know how to calculate \( E(\xi^2) \), so we just need to calculate \( E(\xi)^2 \). We can do this by finding the first derivative of \( G_{\xi}(x) \):

\[ G'_{\xi}(x) = \sum_{i=0}^{\infty} i \cdot P(\xi = i) \cdot x^{i-1} \]

Then if we replace $x$ with $1$ we get:

\[ G'_{\xi}(1) = \sum_{i=0}^{\infty} i \cdot P(\xi = i) \cdot 1^{i-1} = \sum_{i=0}^{\infty} i \cdot P(\xi = i) = E(\xi) \]

So we get:

\[ E(\xi)^2 = G'_{\xi}(1) \cdot G'_{\xi}(1) \]

Then we can calculate the dispersion as:

\[ D(\xi) = E(\xi^2) - E(\xi)^2 = G'_{\xi}(1) + G''_{\xi}(1) - G'_{\xi}(1) \cdot G'_{\xi}(1) \]