\textbf{Problem 1:}

\singlespacing

$f(x) = \text{exp}(-\frac{1}{2\sigma^2}(x - \mu)^2)$

\singlespacing

$f'(x) = (\text{exp}(-\frac{1}{2\sigma^2}(x - \mu)^2))'$

\singlespacing
Applying Chain Rule and $(\text{exp}(x))' = \text{exp}(x)$:
\singlespacing

$f'(x) = \text{exp}(-\frac{1}{2\sigma^2}(x - \mu)^2) (-\frac{1}{2\sigma^2}(x - \mu)^2)'$

\singlespacing

Applying Constant Rule:

\singlespacing

$f'(x) = \text{exp}(-\frac{1}{2\sigma^2}(x - \mu)^2) \cdot -\frac{1}{2\sigma^2}((x - \mu)^2)'$

\singlespacing
Applying Chain Rule and $(x^2)' = 2x$:
\singlespacing

$f'(x) = \text{exp}(-\frac{1}{2\sigma^2}(x - \mu)^2) \cdot -\frac{1}{2\sigma^2}\cdot2(x - \mu) (x - \mu)'$

\singlespacing

Applying Sum Rule

\singlespacing

$f'(x) = \text{exp}(-\frac{1}{2\sigma^2}(x - \mu)^2) \cdot -\frac{1}{2\sigma^2}\cdot2(x - \mu) (x' + (- \mu)')$

\singlespacing

Applying Constant Rule and $(x)' = 1$:

\singlespacing

$f'(x) = \text{exp}(-\frac{1}{2\sigma^2}(x - \mu)^2) \cdot -\frac{1}{2\sigma^2}\cdot2(x - \mu) (1 + 0)$

\singlespacing

$f'(x) = \text{exp}(-\frac{1}{2\sigma^2}(x - \mu)^2) \cdot -\frac{1}{2\sigma^2}\cdot2(x - \mu)$